coq/hm-soundness/HMTypeSafety.v
@@ -1,117 +1,204 @@
 From Coq Require Import Bool.Bool Arith.PeanoNat Lists.List.
 Import ListNotations.
 
+(*
+  Type safety for a polymorphic core language.
+
+  What changed with respect to the first version of this file
+  -----------------------------------------------------------
+  The earlier development called itself Hindley-Milner but its types were
+
+      Inductive ty := TInt | TArrow : ty -> ty -> ty.
+
+  -- no type variables at all.  Lambdas carried an explicit annotation and
+  [let] was monomorphic, so what was proved was the type safety of the simply
+  typed lambda calculus with let and addition.  Nothing polymorphic occurred
+  anywhere.
+
+  Here types have variables, environments map to type schemes, and [let] is
+  polymorphic: the bound expression is required to be typeable at every
+  instance of the scheme, and each occurrence of the bound variable may pick a
+  different instance.  Lambdas lost their annotation (Curry style), so the
+  language is the untyped calculus typed by the relation, as in a real HM
+  system.  [poly_program] below is a program that is typeable here and is not
+  typeable in the monomorphic system, which is what makes the extension real
+  rather than cosmetic.
+
+  Quantified variables are de Bruijn indices ([TBound]) drawn from a
+  constructor distinct from free variables ([TFree]).  Instantiation replaces
+  only [TBound], and the types substituted in contain only [TFree], so variable
+  capture cannot arise and no freshness side conditions are needed.  This is
+  what keeps the development short enough to be checked end to end.
+
+  Generalisation is given semantically: the [TyLet] rule asks that [e1] be
+  typeable at every instance of the scheme, rather than computing the scheme
+  from the free variables of the environment as HMSoundness.v does.  The two
+  files therefore treat generalisation from the two standard angles: the
+  syntactic side condition there, typeability at all instances here.
+*)
+
+(* ------------------------------------------------------------------ *)
+(* Types and schemes                                                   *)
+(* ------------------------------------------------------------------ *)
+
 Inductive ty : Type :=
 | TInt : ty
+| TFree : nat -> ty          (* a free type variable *)
+| TBound : nat -> ty         (* a variable bound by the enclosing scheme *)
 | TArrow : ty -> ty -> ty.
 
-Inductive tm : Type :=
-| TVar : nat -> tm
-| TIntLit : nat -> tm
-| TAdd : tm -> tm -> tm
-| TLam : nat -> ty -> tm -> tm
-| TApp : tm -> tm -> tm
-| TLet : nat -> tm -> tm -> tm.
+(* [Sch n T] is  forall a_0 ... a_{n-1}. T,
+   where a_i occurs in T as [TBound i]. *)
+Inductive scheme : Type :=
+| Sch : nat -> ty -> scheme.
 
-Definition env := nat -> option ty.
-Definition empty : env := fun _ => None.
-Definition extend (G : env) (x : nat) (T : ty) : env :=
-  fun y => if Nat.eqb x y then Some T else G y.
+Definition Mono (T : ty) : scheme := Sch 0 T.
 
-Lemma extend_eq :
-  forall G x T, extend G x T x = Some T.
+(* Instantiation replaces the bound indices by the given types. *)
+Fixpoint open (ts : list ty) (T : ty) : ty :=
+  match T with
+  | TInt => TInt
+  | TFree a => TFree a
+  | TBound i => nth i ts (TBound i)
+  | TArrow A B => TArrow (open ts A) (open ts B)
+  end.
+
+Lemma open_nil : forall T, open [] T = T.
 Proof.
-  intros. unfold extend. now rewrite Nat.eqb_refl.
+  induction T; simpl; try reflexivity.
+  - destruct n; reflexivity.
+  - rewrite IHT1, IHT2. reflexivity.
 Qed.
 
-Lemma extend_neq :
-  forall G x y T, x <> y -> extend G x T y = G y.
+Inductive inst : scheme -> ty -> Prop :=
+| Inst :
+    forall n T ts,
+      length ts = n ->
+      inst (Sch n T) (open ts T).
+
+Lemma inst_mono : forall T, inst (Mono T) T.
 Proof.
-  intros. unfold extend.
+  intros T. unfold Mono.
+  pose proof (Inst 0 T [] eq_refl) as H.
+  rewrite open_nil in H. exact H.
+Qed.
+
+Lemma inst_mono_inv : forall T T', inst (Mono T) T' -> T' = T.
+Proof.
+  intros T T' H. unfold Mono in H. inversion H; subst.
+  match goal with
+  | Hl : length ?l = 0 |- _ =>
+      apply length_zero_iff_nil in Hl; subst; apply open_nil
+  end.
+Qed.
+
+(* ------------------------------------------------------------------ *)
+(* Terms                                                               *)
+(* ------------------------------------------------------------------ *)
+
+Inductive tm : Type :=
+| TmVar : nat -> tm
+| TmInt : nat -> tm
+| TmAdd : tm -> tm -> tm
+| TmLam : nat -> tm -> tm          (* no type annotation: Curry style *)
+| TmApp : tm -> tm -> tm
+| TmLet : nat -> tm -> tm -> tm.
+
+Definition env := nat -> option scheme.
+Definition empty : env := fun _ => None.
+Definition extend (G : env) (x : nat) (Sg : scheme) : env :=
+  fun y => if Nat.eqb x y then Some Sg else G y.
+
+Lemma extend_eq : forall G x Sg, extend G x Sg x = Some Sg.
+Proof. intros. unfold extend. now rewrite Nat.eqb_refl. Qed.
+
+Lemma extend_neq : forall G x y Sg, x <> y -> extend G x Sg y = G y.
+Proof.
+  intros G x y Sg H. unfold extend.
   destruct (Nat.eqb x y) eqn:E.
   - apply Nat.eqb_eq in E. contradiction.
   - reflexivity.
 Qed.
 
+Lemma extend_shadow :
+  forall G x S1 S2, forall y, extend (extend G x S1) x S2 y = extend G x S2 y.
+Proof.
+  intros G x S1 S2 y. unfold extend. destruct (Nat.eqb x y); reflexivity.
+Qed.
+
+Lemma extend_permute :
+  forall G x y Sx Sy,
+    x <> y ->
+    forall z, extend (extend G x Sx) y Sy z = extend (extend G y Sy) x Sx z.
+Proof.
+  intros G x y Sx Sy Hneq z. unfold extend.
+  destruct (Nat.eqb y z) eqn:Eyz; destruct (Nat.eqb x z) eqn:Exz; auto.
+  apply Nat.eqb_eq in Eyz. apply Nat.eqb_eq in Exz. subst. contradiction.
+Qed.
+
+(* ------------------------------------------------------------------ *)
+(* Typing                                                              *)
+(* ------------------------------------------------------------------ *)
+
 Inductive has_type : env -> tm -> ty -> Prop :=
 | TyVar :
-    forall G x T,
-      G x = Some T ->
-      has_type G (TVar x) T
+    forall G x Sg T,
+      G x = Some Sg ->
+      inst Sg T ->
+      has_type G (TmVar x) T
 | TyInt :
     forall G n,
-      has_type G (TIntLit n) TInt
+      has_type G (TmInt n) TInt
 | TyAdd :
     forall G a b,
       has_type G a TInt ->
       has_type G b TInt ->
-      has_type G (TAdd a b) TInt
+      has_type G (TmAdd a b) TInt
 | TyLam :
-    forall G x TArg body TBody,
-      has_type (extend G x TArg) body TBody ->
-      has_type G (TLam x TArg body) (TArrow TArg TBody)
+    forall G x body T1 T2,
+      has_type (extend G x (Mono T1)) body T2 ->
+      has_type G (TmLam x body) (TArrow T1 T2)
 | TyApp :
-    forall G f a TArg TBody,
-      has_type G f (TArrow TArg TBody) ->
-      has_type G a TArg ->
-      has_type G (TApp f a) TBody
+    forall G f a T1 T2,
+      has_type G f (TArrow T1 T2) ->
+      has_type G a T1 ->
+      has_type G (TmApp f a) T2
+(* Polymorphic let: e1 must be typeable at every instance of the scheme,
+   and the body may use x at any of them. *)
 | TyLet :
-    forall G x e1 e2 T1 T2,
-      has_type G e1 T1 ->
-      has_type (extend G x T1) e2 T2 ->
-      has_type G (TLet x e1 e2) T2.
+    forall G x e1 e2 n T0 T2,
+      (forall ts, length ts = n -> has_type G e1 (open ts T0)) ->
+      has_type (extend G x (Sch n T0)) e2 T2 ->
+      has_type G (TmLet x e1 e2) T2.
 
 Inductive value : tm -> Prop :=
-| VInt : forall n, value (TIntLit n)
-| VLam : forall x T body, value (TLam x T body).
+| VInt : forall n, value (TmInt n)
+| VLam : forall x body, value (TmLam x body).
 
 Fixpoint subst (x : nat) (s : tm) (t : tm) : tm :=
   match t with
-  | TVar y => if Nat.eqb x y then s else TVar y
-  | TIntLit n => TIntLit n
-  | TAdd a b => TAdd (subst x s a) (subst x s b)
-  | TLam y T body =>
-      if Nat.eqb x y then TLam y T body else TLam y T (subst x s body)
-  | TApp f a => TApp (subst x s f) (subst x s a)
-  | TLet y e1 e2 =>
-      TLet y (subst x s e1)
-        (if Nat.eqb x y then e2 else subst x s e2)
+  | TmVar y => if Nat.eqb x y then s else TmVar y
+  | TmInt n => TmInt n
+  | TmAdd a b => TmAdd (subst x s a) (subst x s b)
+  | TmLam y body => if Nat.eqb x y then TmLam y body else TmLam y (subst x s body)
+  | TmApp f a => TmApp (subst x s f) (subst x s a)
+  | TmLet y e1 e2 =>
+      TmLet y (subst x s e1) (if Nat.eqb x y then e2 else subst x s e2)
   end.
 
 Inductive step : tm -> tm -> Prop :=
-| ST_AddInts :
-    forall n m,
-      step (TAdd (TIntLit n) (TIntLit m)) (TIntLit (n + m))
-| ST_Add1 :
-    forall a a' b,
-      step a a' ->
-      step (TAdd a b) (TAdd a' b)
-| ST_Add2 :
-    forall v a a',
-      value v ->
-      step a a' ->
-      step (TAdd v a) (TAdd v a')
-| ST_AppLam :
-    forall x T body v,
-      value v ->
-      step (TApp (TLam x T body) v) (subst x v body)
-| ST_App1 :
-    forall f f' a,
-      step f f' ->
-      step (TApp f a) (TApp f' a)
-| ST_App2 :
-    forall v a a',
-      value v ->
-      step a a' ->
-      step (TApp v a) (TApp v a')
-| ST_LetValue :
-    forall x v body,
-      value v ->
-      step (TLet x v body) (subst x v body)
-| ST_Let1 :
-    forall x e1 e1' e2,
-      step e1 e1' ->
-      step (TLet x e1 e2) (TLet x e1' e2).
+| ST_AddInts : forall n m, step (TmAdd (TmInt n) (TmInt m)) (TmInt (n + m))
+| ST_Add1 : forall a a' b, step a a' -> step (TmAdd a b) (TmAdd a' b)
+| ST_Add2 : forall v a a', value v -> step a a' -> step (TmAdd v a) (TmAdd v a')
+| ST_AppLam : forall x body v, value v -> step (TmApp (TmLam x body) v) (subst x v body)
+| ST_App1 : forall f f' a, step f f' -> step (TmApp f a) (TmApp f' a)
+| ST_App2 : forall v a a', value v -> step a a' -> step (TmApp v a) (TmApp v a')
+| ST_LetValue : forall x v body, value v -> step (TmLet x v body) (subst x v body)
+| ST_Let1 : forall x e1 e1' e2, step e1 e1' -> step (TmLet x e1 e2) (TmLet x e1' e2).
+
+(* ------------------------------------------------------------------ *)
+(* Structural lemmas about the environment                             *)
+(* ------------------------------------------------------------------ *)
 
 Lemma context_invariance :
   forall G G' t T,
@@ -119,24 +206,22 @@ Lemma context_invariance :
     has_type G t T ->
     has_type G' t T.
 Proof.
-  intros G G' t T Heq H.
-  generalize dependent G'.
+  intros G G' t T Heq H. generalize dependent G'.
   induction H; intros G' Heq.
-  - apply TyVar. now rewrite <- Heq.
+  - eapply TyVar; [ rewrite <- Heq; eassumption | assumption ].
   - constructor.
   - constructor; auto.
-  - apply TyLam.
-    apply IHhas_type. intros y.
+  - apply TyLam. apply IHhas_type. intros y.
     unfold extend. destruct (Nat.eqb x y); auto.
   - eapply TyApp; eauto.
   - eapply TyLet.
-    + apply IHhas_type1. exact Heq.
-    + apply IHhas_type2. intros y.
+    + intros ts Hlen. apply H0; [ exact Hlen | exact Heq ].
+    + apply IHhas_type. intros y.
       unfold extend. destruct (Nat.eqb x y); auto.
 Qed.
 
 Definition env_extends (G G' : env) : Prop :=
-  forall x T, G x = Some T -> G' x = Some T.
+  forall x Sg, G x = Some Sg -> G' x = Some Sg.
 
 Lemma weakening :
   forall G G' t T,
@@ -144,267 +229,243 @@ Lemma weakening :
     has_type G t T ->
     has_type G' t T.
 Proof.
-  intros G G' t T Hext Hty.
-  generalize dependent G'.
+  intros G G' t T Hext Hty. generalize dependent G'.
   induction Hty; intros G' Hext.
-  - apply TyVar. eauto.
+  - eapply TyVar; [ apply Hext; eassumption | assumption ].
   - constructor.
   - constructor; auto.
-  - apply TyLam.
-    apply IHHty. unfold env_extends in *.
-    intros y Ty Hy.
-    unfold extend in *.
+  - apply TyLam. apply IHHty. unfold env_extends in *.
+    intros y Ty Hy. unfold extend in *.
     destruct (Nat.eqb x y); eauto.
   - eapply TyApp; eauto.
   - eapply TyLet.
-    + apply IHHty1. exact Hext.
-    + apply IHHty2. unfold env_extends in *.
-      intros y Ty Hy.
-      unfold extend in *.
+    + intros ts Hlen. apply H0; [ exact Hlen | exact Hext ].
+    + apply IHHty. unfold env_extends in *.
+      intros y Ty Hy. unfold extend in *.
       destruct (Nat.eqb x y); eauto.
 Qed.
 
 Lemma weaken_empty :
-  forall G t T,
-    has_type empty t T ->
-    has_type G t T.
+  forall G t T, has_type empty t T -> has_type G t T.
 Proof.
-  intros G t T H.
-  eapply weakening; eauto.
-  unfold env_extends, empty.
-  intros x Ty Hnone. discriminate Hnone.
+  intros G t T H. eapply weakening; eauto.
+  unfold env_extends, empty. intros x Ty Hnone. discriminate Hnone.
 Qed.
 
-Lemma extend_shadow :
-  forall G x T1 T2,
-    (forall y, extend (extend G x T1) x T2 y = extend G x T2 y).
-Proof.
-  intros G x T1 T2 y. unfold extend.
-  destruct (Nat.eqb x y); reflexivity.
-Qed.
+(* ------------------------------------------------------------------ *)
+(* Substitution                                                        *)
+(* ------------------------------------------------------------------ *)
 
-Lemma extend_permute :
-  forall G x y Tx Ty,
-    x <> y ->
-    (forall z, extend (extend G x Tx) y Ty z = extend (extend G y Ty) x Tx z).
-Proof.
-  intros G x y Tx Ty Hneq z.
-  unfold extend.
-  destruct (Nat.eqb y z) eqn:Eyz; destruct (Nat.eqb x z) eqn:Exz; auto.
-  apply Nat.eqb_eq in Eyz.
-  apply Nat.eqb_eq in Exz.
-  subst. contradiction.
-Qed.
-
+(* The substituted value must be typeable at every instance of the scheme the
+   variable was bound with.  For a monomorphic binding that is one type; for a
+   let binding it is the whole family. *)
 Lemma substitution_preserves_typing :
-  forall G x U t v T,
-    has_type (extend G x U) t T ->
-    has_type empty v U ->
+  forall t G x Sg v T,
+    has_type (extend G x Sg) t T ->
+    (forall T', inst Sg T' -> has_type empty v T') ->
     has_type G (subst x v t) T.
 Proof.
-  intros G x U t v T Ht Hv.
-  generalize dependent G.
-  generalize dependent T.
-  induction t; intros T G Ht; simpl; inversion Ht; subst.
-  - destruct (Nat.eqb x n) eqn:Exn.
+  induction t; intros G x Sg v T Ht Hv; simpl; inversion Ht; subst.
+  - (* TmVar *)
+    destruct (Nat.eqb x n) eqn:Exn.
     + apply Nat.eqb_eq in Exn. subst.
-      rewrite extend_eq in H1. inversion H1; subst.
-      apply weaken_empty. exact Hv.
-    + apply TyVar.
-      apply Nat.eqb_neq in Exn.
-      rewrite extend_neq in H1 by auto. exact H1.
-  - constructor.
-  - constructor.
-    + eapply IHt1; eauto.
-    + eapply IHt2; eauto.
-  - destruct (Nat.eqb x n) eqn:Exn.
-    + apply TyLam.
-      apply context_invariance with (G := extend (extend G x U) n t).
-      * apply Nat.eqb_eq in Exn. subst.
-        apply extend_shadow.
+      match goal with
+      | Hl : extend _ _ _ _ = Some _ |- _ =>
+          rewrite extend_eq in Hl; inversion Hl; subst
+      end.
+      apply weaken_empty. apply Hv.
+      match goal with | Hi : inst _ _ |- _ => exact Hi end.
+    + apply Nat.eqb_neq in Exn.
+      eapply TyVar.
       * match goal with
-        | Hbody : has_type (extend (extend G x U) n t) _ _ |- _ => exact Hbody
+        | Hl : extend _ _ _ _ = Some _ |- _ =>
+            rewrite extend_neq in Hl by auto; exact Hl
         end.
-    + apply TyLam.
-      apply IHt.
-      apply context_invariance with (G := extend (extend G x U) n t).
-      * apply Nat.eqb_neq in Exn.
-        apply extend_permute. exact Exn.
-      * match goal with
-        | Hbody : has_type (extend (extend G x U) n t) _ _ |- _ => exact Hbody
-        end.
-  - eapply TyApp.
-    + eapply IHt1; eauto.
-    + eapply IHt2; eauto.
-  - eapply TyLet.
-    + eapply IHt1; eauto.
+      * match goal with | Hi : inst _ _ |- _ => exact Hi end.
+  - (* TmInt *)
+    constructor.
+  - (* TmAdd *)
+    constructor; [ eapply IHt1 | eapply IHt2 ]; eauto.
+  - (* TmLam *)
+    destruct (Nat.eqb x n) eqn:Exn.
+    + apply Nat.eqb_eq in Exn. subst.
+      apply TyLam.
+      apply context_invariance with (G := extend (extend G n Sg) n (Mono T1)).
+      * apply extend_shadow.
+      * assumption.
+    + apply Nat.eqb_neq in Exn.
+      apply TyLam. eapply IHt with (Sg := Sg); [ | exact Hv ].
+      apply context_invariance with (G := extend (extend G x Sg) n (Mono T1)).
+      * apply extend_permute. exact Exn.
+      * assumption.
+  - (* TmApp *)
+    eapply TyApp; [ eapply IHt1 | eapply IHt2 ]; eauto.
+  - (* TmLet *)
+    eapply TyLet.
+    + intros ts Hlen. eapply IHt1 with (Sg := Sg); [ | exact Hv ].
+      match goal with
+      | Hp : forall l : list ty, _ |- _ => apply Hp; exact Hlen
+      end.
     + destruct (Nat.eqb x n) eqn:Exn.
-      * apply context_invariance with (G := extend (extend G x U) n T1).
-        -- apply Nat.eqb_eq in Exn. subst.
-           apply extend_shadow.
-        -- match goal with
-           | Hbody : has_type (extend (extend G x U) n T1) _ _ |- _ => exact Hbody
-           end.
-      * apply IHt2.
-        apply context_invariance with (G := extend (extend G x U) n T1).
-        -- apply Nat.eqb_neq in Exn.
-           apply extend_permute. exact Exn.
-        -- match goal with
-           | Hbody : has_type (extend (extend G x U) n T1) _ _ |- _ => exact Hbody
-           end.
+      * apply Nat.eqb_eq in Exn. subst.
+        apply context_invariance with (G := extend (extend G n Sg) n (Sch n0 T0)).
+        -- apply extend_shadow.
+        -- assumption.
+      * apply Nat.eqb_neq in Exn.
+        eapply IHt2 with (Sg := Sg); [ | exact Hv ].
+        apply context_invariance with (G := extend (extend G x Sg) n (Sch n0 T0)).
+        -- apply extend_permute. exact Exn.
+        -- assumption.
 Qed.
 
+(* ------------------------------------------------------------------ *)
+(* Canonical forms                                                     *)
+(* ------------------------------------------------------------------ *)
+
 Lemma canonical_int :
-  forall v,
-    value v ->
-    has_type empty v TInt ->
-    exists n, v = TIntLit n.
+  forall v, value v -> has_type empty v TInt -> exists n, v = TmInt n.
 Proof.
-  intros v Hv Ht. inversion Hv; subst; eauto.
-  inversion Ht.
+  intros v Hv Ht. inversion Hv; subst; eauto. inversion Ht.
 Qed.
 
 Lemma canonical_arrow :
   forall v T1 T2,
-    value v ->
-    has_type empty v (TArrow T1 T2) ->
-    exists x body, v = TLam x T1 body.
+    value v -> has_type empty v (TArrow T1 T2) -> exists x body, v = TmLam x body.
 Proof.
   intros v T1 T2 Hv Ht. inversion Hv; subst.
   - inversion Ht.
-  - inversion Ht; subst. eauto.
+  - eauto.
 Qed.
 
+(* ------------------------------------------------------------------ *)
+(* Progress and preservation                                           *)
+(* ------------------------------------------------------------------ *)
+
 Theorem progress :
-  forall t T,
-    has_type empty t T ->
-    value t \/ exists t', step t t'.
+  forall t T, has_type empty t T -> value t \/ exists t', step t t'.
 Proof.
-  intros t T Ht.
-  remember empty as G.
-  induction Ht; subst.
-  - discriminate.
+  intros t T Ht. remember empty as G. induction Ht; subst.
+  - (* TmVar: impossible in the empty environment *)
+    unfold empty in H. discriminate.
   - left. constructor.
   - right.
     destruct IHHt1 as [Hv1 | [a' Ha']]; auto.
     + destruct IHHt2 as [Hv2 | [b' Hb']]; auto.
       * destruct (canonical_int a Hv1 Ht1) as [n ->].
         destruct (canonical_int b Hv2 Ht2) as [m ->].
-        exists (TIntLit (n + m)). constructor.
-      * exists (TAdd a b'). constructor; auto.
-    + exists (TAdd a' b). constructor; auto.
+        exists (TmInt (n + m)). constructor.
+      * exists (TmAdd a b'). constructor; auto.
+    + exists (TmAdd a' b). constructor; auto.
   - left. constructor.
   - destruct IHHt1 as [Hvf | [f' Hf']]; auto.
     + destruct IHHt2 as [Hva | [a' Ha']]; auto.
-      * right.
-        destruct (canonical_arrow f TArg TBody Hvf Ht1) as [x [body ->]].
+      * right. destruct (canonical_arrow f T1 T2 Hvf Ht1) as [x [body ->]].
         exists (subst x a body). constructor; auto.
-      * right. exists (TApp f a'). constructor; auto.
-    + right. exists (TApp f' a). constructor; auto.
-  - destruct IHHt1 as [Hv1 | [e1' He1']]; auto.
+      * right. exists (TmApp f a'). constructor; auto.
+    + right. exists (TmApp f' a). constructor; auto.
+  - (* TmLet: use the instance at a list of the right length *)
+    assert (Hlen : length (repeat TInt n) = n) by apply repeat_length.
+    destruct (H0 (repeat TInt n) Hlen eq_refl) as [Hv1 | [e1' He1']].
     + right. exists (subst x e1 e2). constructor; auto.
-    + right. exists (TLet x e1' e2). constructor; auto.
+    + right. exists (TmLet x e1' e2). constructor; auto.
 Qed.
 
 Theorem preservation :
-  forall t t' T,
-    has_type empty t T ->
-    step t t' ->
-    has_type empty t' T.
+  forall t t' T, has_type empty t T -> step t t' -> has_type empty t' T.
 Proof.
-  intros t t' T Ht Hs.
-  generalize dependent T.
+  intros t t' T Ht Hs. generalize dependent T.
   induction Hs; intros T0 Ht; inversion Ht; subst.
   - constructor.
-  - constructor.
-    + apply IHHs.
-      match goal with
-      | H : has_type empty a _ |- _ => exact H
-      end.
-    + match goal with
-      | H : has_type empty b TInt |- _ => exact H
-      end.
-  - constructor.
-    + match goal with
-      | H : has_type empty v TInt |- _ => exact H
-      end.
-    + apply IHHs.
-      match goal with
-      | H : has_type empty a TInt |- _ => exact H
-      end.
-  - match goal with
-    | Hfun : has_type empty (TLam x T body) (TArrow _ _) |- _ =>
-        inversion Hfun; subst
+  - constructor; [ apply IHHs; assumption | assumption ].
+  - constructor; [ assumption | apply IHHs; assumption ].
+  - (* beta *)
+    match goal with
+    | Hfun : has_type empty (TmLam x body) (TArrow _ _) |- _ => inversion Hfun; subst
     end.
-    eapply substitution_preserves_typing; eauto.
-  - eapply TyApp.
-    + apply IHHs.
+    eapply substitution_preserves_typing; [ eassumption | ].
+    intros T' Hi. apply inst_mono_inv in Hi. subst. assumption.
+  - eapply TyApp; [ apply IHHs; eassumption | eassumption ].
+  - eapply TyApp; [ eassumption | apply IHHs; eassumption ].
+  - (* let of a value *)
+    eapply substitution_preserves_typing; [ eassumption | ].
+    intros T' Hi. inversion Hi; subst.
+    match goal with
+    | Hp : forall l : list ty, _ |- _ => apply Hp; reflexivity
+    end.
+  - (* let, evaluating the bound expression *)
+    econstructor.
+    + intros ts Hlen. apply IHHs.
       match goal with
-      | H : has_type empty f _ |- _ => exact H
+      | Hp : forall l : list ty, _ |- _ => apply Hp; exact Hlen
       end.
-    + match goal with
-      | H : has_type empty a _ |- _ => exact H
-      end.
-  - eapply TyApp.
-    + match goal with
-      | H : has_type empty v _ |- _ => exact H
-      end.
-    + apply IHHs.
-      match goal with
-      | H : has_type empty a _ |- _ => exact H
-      end.
-  - eapply substitution_preserves_typing; eauto.
-  - eapply TyLet.
-    + apply IHHs.
-      match goal with
-      | H : has_type empty e1 _ |- _ => exact H
-      end.
-    + match goal with
-      | H : has_type (extend empty x _) e2 _ |- _ => exact H
-      end.
+    + eassumption.
 Qed.
 
 Theorem type_safety :
-  forall t t' T,
-    has_type empty t T ->
-    step t t' ->
-    has_type empty t' T.
+  forall t t' T, has_type empty t T -> step t t' -> has_type empty t' T.
+Proof. apply preservation. Qed.
+
+(* ------------------------------------------------------------------ *)
+(* The polymorphism is real                                            *)
+(* ------------------------------------------------------------------ *)
+
+Definition id_tm : tm := TmLam 0 (TmVar 0).
+
+(* id has the scheme  forall a. a -> a  *)
+Definition id_scheme : scheme := Sch 1 (TArrow (TBound 0) (TBound 0)).
+
+Lemma id_at_every_instance :
+  forall ts, length ts = 1 -> has_type empty id_tm (open ts (TArrow (TBound 0) (TBound 0))).
 Proof.
-  apply preservation.
+  intros ts Hlen. destruct ts as [| t ts']; simpl in Hlen; try discriminate.
+  destruct ts' as [| u ts'']; simpl in Hlen; try discriminate.
+  simpl. unfold id_tm. apply TyLam.
+  eapply TyVar; [ apply extend_eq | apply inst_mono ].
 Qed.
 
-Definition plus_one : tm :=
-  TLam 0 TInt (TAdd (TVar 0) (TIntLit 1)).
+(*  let id = fun x -> x in (id id) 42
+    The first occurrence of id is used at (int -> int) -> (int -> int),
+    the second at int -> int.  A monomorphic let cannot type this. *)
+Definition poly_program : tm :=
+  TmLet 1 id_tm (TmApp (TmApp (TmVar 1) (TmVar 1)) (TmInt 42)).
 
-Definition sample_program : tm :=
-  TLet 1 plus_one (TApp (TVar 1) (TIntLit 41)).
-
-Lemma sample_program_typed :
-  has_type empty sample_program TInt.
+Lemma poly_program_typed :
+  has_type empty poly_program TInt.
 Proof.
-  unfold sample_program, plus_one.
-  eapply TyLet with (T1 := TArrow TInt TInt).
-  - apply TyLam.
-    constructor.
-    + apply TyVar. apply extend_eq.
-    + constructor.
-  - eapply TyApp with (TArg := TInt).
-    + apply TyVar. apply extend_eq.
+  unfold poly_program.
+  eapply TyLet with (n := 1) (T0 := TArrow (TBound 0) (TBound 0)).
+  - apply id_at_every_instance.
+  - eapply TyApp with (T1 := TInt).
+    + eapply TyApp with (T1 := TArrow TInt TInt).
+      * eapply TyVar; [ apply extend_eq | ].
+        pose proof (Inst 1 (TArrow (TBound 0) (TBound 0))
+                         [TArrow TInt TInt] eq_refl) as H.
+        simpl in H. exact H.
+      * eapply TyVar; [ apply extend_eq | ].
+        pose proof (Inst 1 (TArrow (TBound 0) (TBound 0)) [TInt] eq_refl) as H.
+        simpl in H. exact H.
     + constructor.
 Qed.
 
-Lemma sample_program_steps :
-  exists t',
-    step sample_program t' /\ has_type empty t' TInt.
+(* The same program is not typeable if the binding is kept monomorphic:
+   the two occurrences would have to receive the same type. *)
+Lemma poly_program_needs_polymorphism :
+  forall T,
+    inst (Mono T) (TArrow (TArrow TInt TInt) (TArrow TInt TInt)) ->
+    inst (Mono T) (TArrow TInt TInt) ->
+    False.
 Proof.
-  exists (subst 1 plus_one (TApp (TVar 1) (TIntLit 41))).
+  intros T H1 H2.
+  apply inst_mono_inv in H1. apply inst_mono_inv in H2. subst. discriminate.
+Qed.
+
+Lemma poly_program_steps :
+  exists t', step poly_program t' /\ has_type empty t' TInt.
+Proof.
+  exists (subst 1 id_tm (TmApp (TmApp (TmVar 1) (TmVar 1)) (TmInt 42))).
   split.
-  - unfold sample_program.
-    apply ST_LetValue.
-    unfold plus_one. constructor.
+  - unfold poly_program. apply ST_LetValue. unfold id_tm. constructor.
   - eapply preservation.
-    + apply sample_program_typed.
-    + unfold sample_program.
-      apply ST_LetValue.
-      unfold plus_one. constructor.
+    + apply poly_program_typed.
+    + unfold poly_program. apply ST_LetValue. unfold id_tm. constructor.
 Qed.
